wip

src/matroid/quotients.lean
@@ -7,12 +7,11 @@ open set list
 
 namespace matroid
 
-variables {E : Type*} [finite E] {X Y I C B F : set E} {N M : matroid E} {e f : E}
+variables {E : Type*} {X Y I C B F : set E} {N M : matroid E} {e f : E}
 
 section weak_image
 /- `M` is a weak image of `N` if independence in `N` implies independence in `M` -/
-def weak_image (N M : matroid E) :=
-  ∀ I, N.indep I → M.indep I
+def weak_image (N M : matroid E) := ∀ I, N.indep I → M.indep I
 
 -- instance weak_image_le : has_le (matroid E) :=
 -- ⟨λ N M, is_weak_image N M⟩
@@ -24,21 +23,20 @@ lemma weak_image_def : N ≤w M ↔ ∀ I, N.indep I → M.indep I := iff.rfl
 
 lemma indep.weak_image (hI : N.indep I) (h : N ≤w M) : M.indep I := h _ hI
 
-lemma weak_image_iff_r : N ≤w M ↔ ∀ X, N.r X ≤ M.r X :=
-begin
+lemma weak_image_iff_r [finite_rk N] [finite_rk M] : N ≤w M ↔ ∀ X, N.r X ≤ M.r X :=
+begin 
   simp_rw [r_le_iff, le_r_iff],
   refine ⟨λ h X I hIX hIN, ⟨I, hIX, h _ hIN, rfl⟩, λ h I hI, _⟩,
   obtain ⟨J,hJI,hJ,hJ'⟩ := h I I subset.rfl hI,
-  rwa [←eq_of_subset_of_ncard_le hJI hJ'.symm.le],
+  rwa [←eq_of_subset_of_ncard_le hJI hJ'.symm.le hI.finite],
 end
 
-lemma weak_image.r_le (h : N ≤w M) (X : set E) : N.r X ≤ M.r X := weak_image_iff_r.mp h X
+lemma weak_image.r_le [finite_rk N] [finite_rk M] (h : N ≤w M) (X : set E) : N.r X ≤ M.r X := weak_image_iff_r.mp h X
 
 lemma weak_image_iff_dep : N ≤w M ↔ ∀ X, ¬M.indep X → ¬N.indep X :=
 by simp_rw [weak_image_def, not_imp_not]
 
-lemma weak_image.dep (h : N ≤w M) (hX : ¬M.indep X) : ¬ N.indep X :=
-weak_image_iff_dep.mp h _ hX
+lemma weak_image.dep (h : N ≤w M) (hX : ¬M.indep X) : ¬ N.indep X := weak_image_iff_dep.mp h _ hX
 
 lemma weak_image_iff_circuit : N ≤w M ↔ ∀ C, M.circuit C → ∃ C' ⊆ C, N.circuit C' :=
 begin
@@ -54,7 +52,7 @@ lemma circuit.supset_circuit_of_weak_image (hC : M.circuit C) (h : N ≤w M) :
   ∃ C' ⊆ C, N.circuit C' :=
 weak_image_iff_circuit.mp h _ hC 
 
-lemma weak_image_tfae :
+lemma weak_image_tfae [finite_rk N] [finite_rk M] :
   tfae
 [ N ≤w M,
   ∀ X, N.r X ≤ M.r X,
@@ -69,7 +67,8 @@ begin
   tfae_finish,
 end
 
-lemma weak_image.rank_zero_of_rank_zero (h : N ≤w M) (hX : M.r X = 0) : N.r X = 0 :=
+lemma weak_image.r_eq_zero_of_r_eq_zero [finite_rk N] [finite_rk M] (h : N ≤w M) (hX : M.r X = 0) : 
+  N.r X = 0 :=
 nat.eq_zero_of_le_zero ((weak_image.r_le h X).trans_eq hX)
 
 lemma loop.weak_image (he : M.loop e) (h : N ≤w M) : N.loop e :=
@@ -84,6 +83,12 @@ lemma weak_image.trans {M₀ M₁ M₂ : matroid E} (h₀₁ : M₀ ≤w M₁) (
 lemma weak_image.antisymm (h : M ≤w N) (h' : N ≤w M) : M = N :=
 eq_of_indep_iff_indep_forall (λ I, ⟨λ hI, h I hI, λ hI, h' I hI⟩)
 
+lemma weak_image.finite_rk [finite_rk N] (h : M ≤w N) : finite_rk M := 
+begin
+  obtain ⟨B, hB⟩ := M.exists_base, 
+  exact finite_rk_of_finite_base hB ((hB.indep.weak_image h).finite),
+end 
+
 end weak_image
 
 section quotient
@@ -91,46 +96,16 @@ section quotient
 the corresponding rank differences in M. This is equivalent to the existence of a matroid P for
 which M is a deletion of P and N is a contraction of P, but we do not show this equivalence here.
 -/
-def is_quotient (N M : matroid E) :=
-  ∀ X, M.cl X ⊆ N.cl X
+def is_quotient (N M : matroid E) := ∀ X, M.cl X ⊆ N.cl X
 
 reserve infixl ` ≼ `:75
 infix ` ≼ ` :=  is_quotient
 
-lemma is_quotient.cl_subset (h : N ≼ M) (X : set E) : M.cl X ⊆ N.cl X :=
-h X
-
-lemma is_quotient.r_le_r_of_subset (h : N ≼ M) (hXY : X ⊆ Y) : 
-  (N.r Y : ℤ)  - N.r X ≤ M.r Y - M.r X :=
-begin
-  by_contra' hlt,
-  set P : set E → Prop := λ Z, X ⊆ Z ∧ Z ⊆ Y ∧ (M.r Y : ℤ) - M.r Z < N.r Y - N.r Z,
-  obtain ⟨Z,⟨hXZ,hZY,hlt'⟩,hmax⟩ := finite.exists_maximal P ⟨X, subset.rfl, hXY, hlt⟩,
-  have hss := hZY.ssubset_of_ne (by {rintro rfl, simpa using hlt'}),
-  rw [int.lt_iff_add_one_le, ←le_sub_iff_add_le] at hlt',
-  obtain ⟨e,heY,heZ⟩ := exists_of_ssubset hss,
-
-  refine (insert_ne_self.mpr (heZ)).symm
-      (hmax (insert e Z) ⟨hXZ.trans (set.subset_insert _ _),
-      insert_subset.mpr ⟨heY,hZY⟩, lt_of_not_le (λ hle, _)⟩ (subset_insert _ _)),
-
-  by_cases h₁ : e ∈ M.cl Z,
-  { rw [mem_cl_iff_r_insert.mp h₁, mem_cl_iff_r_insert.mp (h Z h₁)] at hle,  linarith},
-
-  rw [not_mem_cl_iff_r_insert.mp h₁, nat.cast_add, nat.cast_one] at hle,
-  linarith [N.r_insert_le_add_one Z e],
-end
-
-lemma is_quotient_iff_r : N ≼ M ↔ ∀ X Y, X ⊆ Y → (N.r Y : ℤ)  - N.r X ≤ M.r Y - M.r X :=
-begin
-  refine ⟨λ h X Y hXY, h.r_le_r_of_subset hXY, λ h Z e he, _⟩,
-  have hle := h _ _ (subset_insert e Z),
-  rw [mem_cl_iff_r_insert.mp he, sub_self, sub_le_iff_le_add, zero_add, nat.cast_le] at hle,
-  apply mem_cl_of_r_insert_le hle,
-end
+lemma is_quotient.cl_subset (h : N ≼ M) (X : set E) : M.cl X ⊆ N.cl X := h X
 
 lemma is_quotient.weak_image (h : N ≼ M) : N ≤w M :=
 begin
+  
   refine λ X hX, by_contra (λ h', _),
   obtain ⟨C,hCX,hC⟩ := dep_iff_supset_circuit.mp h',
   obtain ⟨e,heC⟩ := hC.nonempty,
@@ -138,14 +113,49 @@ begin
   exact (cl_subset_cl_of_subset_cl he).not_ssubset ((hX.subset hCX).cl_diff_singleton_ssubset heC),
 end
 
-lemma indep.quotient (hI : N.indep I) (h : N ≼ M) : M.indep I :=
-hI.weak_image h.weak_image
+lemma is_quotient.r_le_r_of_subset [finite_rk M] (h : N ≼ M) (hXY : X ⊆ Y) : 
+  (N.r Y : ℤ)  - N.r X ≤ M.r Y - M.r X :=
+begin
+  haveI := h.weak_image.finite_rk, 
+  obtain ⟨IM,hIM⟩ := M.exists_basis X, 
+  obtain ⟨JM,hIJM,hJM⟩ := hIM.indep.subset_basis_of_subset (hIM.subset.trans hXY),  
+  obtain ⟨IN,hIN⟩ := N.exists_basis IM,
+  obtain ⟨JN,hIJN,hJN⟩ := hIN.indep.subset_basis_of_subset (subset_union_left IN (JM \ IM)), 
+  have hINX : N.basis IN X, 
+  { refine hIN.indep.basis_of_subset_cl (hIN.subset.trans hIM.subset) _,
+    rw hIN.cl, 
+    refine subset_trans hIM.subset_cl (h _) },
+  have hJNY : N.basis JN Y, 
+  { refine hJN.indep.basis_of_subset_cl (hJN.subset.trans _) _,
+    { exact union_subset (hIN.subset.trans (hIJM.trans hJM.subset)) 
+      ((diff_subset JM _).trans hJM.subset) },
+    rw [hJN.cl, ←cl_union_cl_left_eq_cl_union, hIN.cl, cl_union_cl_left_eq_cl_union, 
+      union_diff_self, union_eq_right_iff_subset.mpr hIJM],
+    exact hJM.subset_cl.trans (h _) },
+  rw [←hINX.card, ←hJNY.card, ←hJM.card, ←hIM.card, ←ncard_diff_add_ncard_eq_ncard hIJM hJM.finite, 
+    ←ncard_diff_add_ncard_eq_ncard hIJN hJN.finite, nat.cast_add, nat.cast_add, 
+    add_tsub_cancel_right, add_tsub_cancel_right, nat.cast_le],  
+  refine ncard_le_of_subset _ (hJM.finite.diff _), 
+  rw diff_subset_iff, 
+  exact hJN.subset, 
+end
+
+lemma is_quotient_iff_r [finite E] : 
+  N ≼ M ↔ ∀ X Y, X ⊆ Y → (N.r Y : ℤ)  - N.r X ≤ M.r Y - M.r X :=
+begin
+  refine ⟨λ h X Y hXY, h.r_le_r_of_subset hXY, λ h Z e he, _⟩,
+  have hle := h _ _ (subset_insert e Z),
+  rw [mem_cl_iff_r_insert.mp he, sub_self, sub_le_iff_le_add, zero_add, nat.cast_le] at hle,
+  apply mem_cl_of_r_insert_le hle,
+end
+
+lemma indep.quotient (hI : N.indep I) (h : N ≼ M) : M.indep I := hI.weak_image h.weak_image
 
 /- TODO : prove without rank (or with relative rank)-/
-lemma quotient_iff_dual_quotient : N ≼ M ↔ M.dual ≼ N.dual :=
+lemma quotient_iff_dual_quotient [finite E] : N ≼ M ↔ M﹡ ≼ N﹡ :=
 begin
-  suffices h' : ∀ (N M : matroid E), N ≼ M → M.dual ≼ N.dual,
-  exact ⟨λ h, h' _ _ h, λ h, by {convert h' _ _ h; rw dual_dual, }⟩,
+  suffices h' : ∀ (N M : matroid E), N ≼ M → M﹡ ≼ N﹡,
+  exact ⟨λ h, h' _ _ h, λ h, by {convert h' _ _ h; rw dual_dual }⟩,
   simp_rw [is_quotient_iff_r, dual_rank_cast_eq],
   intros N M h X Y hXY,
   have := h _ _ (compl_subset_compl.mpr hXY),
@@ -164,7 +174,7 @@ end
 
 lemma flat.quotient (hF : N.flat F) (h : N ≼ M) : M.flat F := (is_quotient_iff_flat.mp h) F hF
 
-lemma quotient_tfae :
+lemma quotient_tfae [finite E] :
   tfae
 [N ≼ M,
  ∀ F, N.flat F → M.flat F,
@@ -179,9 +189,9 @@ begin
   tfae_finish,
 end
 
-lemma quotient_iff_cl : N ≼ M ↔ ∀ X, M.cl X ⊆ N.cl X := by apply @tfae.out _ quotient_tfae 0 3
+lemma quotient_iff_cl : N ≼ M ↔ ∀ X, M.cl X ⊆ N.cl X := iff.rfl 
 
-lemma eq_of_quotient_of_rk_eq_rk (h : N ≼ M) (hr : N.rk = M.rk) : N = M :=
+lemma eq_of_quotient_of_rk_eq_rk [finite E] (h : N ≼ M) (hr : N.rk = M.rk) : N = M :=
 begin
   refine eq_of_r_eq_r_forall _,
   by_contra' h',
