src/matroid/loop.lean
@@ -22,8 +22,8 @@ lemma loop_iff_mem_cl_empty : M.loop e ↔ e ∈ M.cl ∅ := iff.rfl
 lemma cl_empty_eq_loops (M : matroid E) : M.cl ∅ = {e | M.loop e} := rfl 
 
 lemma loop_iff_dep : M.loop e ↔ ¬ M.indep {e} :=
-by rw [loop_iff_mem_cl_empty, iff_not_comm, M.empty_indep.not_mem_cl_iff, mem_empty_iff_false, 
-    not_false_iff, true_and, insert_emptyc_eq]
+by rw [loop_iff_mem_cl_empty, iff_not_comm, M.empty_indep.not_mem_cl_iff, 
+  mem_empty_iff_false, not_false_iff, true_and, insert_emptyc_eq]
 
 lemma loop_iff_circuit : M.loop e ↔ M.circuit {e} := 
 begin
