src/matroid/pseudominor'.lean
@@ -1,0 +1,1083 @@
+import mathlib.data.set.basic
+import mathlib.order.boolean_algebra
+import .quotients
+import .connectivity
+
+/-!
+# Projections, Loopifications and Pseudominors
+
+For a matroid `M` on Type `E` and sets `C,D` in `M`, this file defines matroids `M ⟋ C` and
+`M ⟍ D` which are obtained from `M` by contracting `C` and deleting `D` respectively, but then
+adding back in `C` (or `D`) as a set containing only loops. We call these operations 'projection'
+and 'loopification'.
+
+The advantage of this over taking minors is that we stay in the Type `matroid E` rather than
+changing the ground set and having to deal with type equality . In practice it seems
+that many proofs that involve manipulating minors can be phrased only in terms of these modified
+minor-like-objects, which we call pseudominors.
+
+Kung's theorem and the matroid intersection theorem are currently both proved in this way.
+(or at least will be once I fix them again)
+-/
+
+noncomputable theory
+open set
+
+section symbols 
+
+@[class] structure has_con (α β : Type*) :=
+(con : α → β → α)
+
+@[class] structure has_restr (α β : Type*) :=
+(restr : α → β → α)
+
+infix ` ⟋ ` :75 :=  has_con.con
+
+-- infix ` ⟍ ` :75 :=  has_del.del 
+
+infix ` ‖ ` :75 :=  has_restr.restr 
+
+end symbols 
+
+variables {E : Type*}  {e f : E} {M N : matroid E} {X Y D C F B I I₀ R : set E}
+
+namespace matroid
+
+section restrict
+
+instance {E : Type*} : has_restr (matroid E) (set E) := ⟨λ M E, M.lrestrict E⟩  
+
+@[simp] lemma restr_indep_iff : (M ‖ X).indep I ↔ M.indep I ∧ I ⊆ X := lrestrict_indep_iff
+
+/-- Restriction is deletion of the complement -/
+-- def has_del.restr {α β : Type*} [has_del α β] [has_compl β] (M : α) (R : β) : α := M ⟍ Rᶜ
+
+-- infix ` ‖ ` :75 :=  has_del.restr
+
+-- lemma restr_eq_del {α β : Type*} [has_del α β] [has_compl β] (M : α) (R : β) : M ‖ R = M ⟍ Rᶜ := 
+-- rfl 
+
+@[simp] lemma lrestrict_r (M : matroid E) (R X : set E) : (M ‖ R).r X = M.r (X ∩ R) :=
+by simp [restr_eq_del]
+
+lemma loopify_eq_lrestrict_compl (M : matroid E) (D : set E) : (M ⟍ D) = (M ‖ Dᶜ) :=
+by rw [restr_eq_del, compl_compl]
+
+lemma loopify_compl_eq_lrestrict (M : matroid E) (D : set E) : M ⟍ Dᶜ = M ‖ D := rfl
+
+lemma lrestrict_nonloop_iff : (M ‖ R).nonloop e ↔ M.nonloop e ∧ e ∈ R :=
+by rw [restr_eq_del, nonloop_loopify_iff, not_mem_compl_iff]   
+
+@[simp] lemma lrestrict.nonloops (M : matroid E) (R : set E) : ((M ‖ R).cl ∅)ᶜ = (M.cl ∅)ᶜ ∩ R :=
+by { ext, simp_rw [mem_inter_iff, mem_compl_iff, ←loop_iff_mem_cl_empty, not_loop_iff, 
+  lrestrict_nonloop_iff] }
+
+@[simp] lemma indep_lrestrict_iff : (M ‖ R).indep I ↔ M.indep I ∧ I ⊆ R :=
+by simp [restr_eq_del, disjoint_compl_right_iff_subset, and_comm]
+
+lemma skew_iff_project_lrestrict_eq_lrestrict :
+  M.skew C R ↔ (M ⟋ C) ‖ R = M ‖ R :=
+begin
+  refine ⟨λ h, _,λ h, _⟩, 
+  { refine eq_of_r_eq_r_forall (λ X, _), 
+    zify, 
+    simp_rw [lrestrict_r, coe_r_project, ←(h.symm.subset_left (inter_subset_right X _)).r_add], 
+    simp only [nat.cast_add, add_tsub_cancel_right] },
+  rw skew_iff_r, 
+  apply_fun (λ M, M.r univ) at h, 
+  zify at *, 
+  rw [lrestrict_r, lrestrict_r, univ_inter, coe_r_project, union_comm] at h, 
+  simp [←h],
+end 
+
+end restrict
+
+section project
+
+/-- contract `C` and replace it with a set of loops to get a matroid on the same ground set.
+Often more convenient than just contracting `C` because the underlying type is preserved. -/
+def project (M : matroid E) (C : set E) :
+  matroid E :=
+matroid_of_cl
+  (λ X, M.cl (X ∪ C))
+  (λ X, (subset_union_left _ _).trans (M.subset_cl _))
+  (λ X Y hXY, M.cl_mono (union_subset_union_left _ hXY))
+  (λ X, by {simp only [cl_union_cl_left_eq_cl_union, union_assoc, union_self]} )
+  (λ X e f hf, by {rw [insert_union] at ⊢ hf, exact cl_exchange hf})
+
+instance {E : Type*} [finite E] : has_con (matroid E) (set E) := ⟨matroid.project⟩  
+instance {E : Type*} [finite E] : has_con (matroid E) E := ⟨λ M e, M.project {e}⟩  
+
+-- @[simp] lemma project_def 
+
+-- infix ` ⟋ ` :75 :=  matroid.project
+
+/-- Project every element outside `R` -/
+def project_to (M : matroid E) (R : set E) : matroid E :=
+  M ⟋ Rᶜ
+
+@[simp] lemma project_cl_eq (M : matroid E) (C X : set E) :
+  (M ⟋ C).cl X = M.cl (X ∪ C) :=
+by simp only [has_con.con, matroid.project, matroid_of_cl_apply]
+
+@[simp] lemma project_empty (M : matroid E) : M ⟋ (∅ : set E) = M :=
+eq_of_cl_eq_cl_forall (λ X, by simp_rw [project_cl_eq, union_empty])
+
+@[simp] lemma project_project (M : matroid E) (C₁ C₂ : set E) :
+  M ⟋ C₁ ⟋ C₂ = M ⟋ (C₁ ∪ C₂) :=
+begin
+  refine eq_of_cl_eq_cl_forall (λ X, _),
+  simp_rw [project_cl_eq],
+  rw [union_right_comm, union_assoc],
+end
+
+lemma project_is_quotient (M : matroid E) (C : set E) :
+  M ⟋ C ≼ M :=
+begin
+  simp_rw [is_quotient, project_cl_eq],
+  exact λ X, M.cl_mono (subset_union_left _ _),
+end
+
+lemma project_weak_image (M : matroid E) (C : set E) :
+  M ⟋ C ≤w M :=
+(M.project_is_quotient C).weak_image
+
+lemma project_project_comm (M : matroid E) (C₁ C₂ : set E) :
+  M ⟋ C₁ ⟋ C₂ = M ⟋ C₂ ⟋ C₁ :=
+by rw [project_project, project_project, union_comm]
+
+lemma project_contract_subset_loops (M : matroid E) (C : set E) :
+  C ⊆ (M ⟋ C).cl ∅ :=
+by {rw [project_cl_eq, empty_union], apply M.subset_cl}
+
+lemma project_indep_disjoint_contract (hI : (M ⟋ C).indep I) :
+  disjoint I C :=
+begin
+  simp_rw [indep_iff_not_mem_cl_diff_forall, project_cl_eq] at hI,
+  rw [disjoint_iff_forall_ne],
+  rintro x hxI _ hxC rfl,
+  exact hI x hxI (M.subset_cl _ (or.inr hxC)),
+end
+
+lemma project_indep_disjoint_cl_contract (hI : (M ⟋ C).indep I) :
+  disjoint I (M.cl C) :=
+begin
+  simp_rw [indep_iff_not_mem_cl_diff_forall, project_cl_eq] at hI,
+  rw [disjoint_iff_forall_ne],
+  rintro x hxI _ hxC rfl,
+  exact hI x hxI (mem_of_mem_of_subset hxC (M.cl_mono (subset_union_right _ _))),
+end
+
+lemma union_indep_of_project_indep (hI : (M ⟋ C).indep I) (hI₀ : M.basis I₀ C) :
+  M.indep (I ∪ I₀) :=
+begin
+  by_contra h',
+  simp_rw [indep_iff_not_mem_cl_diff_forall, project_cl_eq] at hI,
+  rw dep_iff_supset_circuit at h',
+  obtain ⟨D,hDss,hD⟩ := h',
+
+  have heD : (D ∩ I).nonempty,
+  { rw [nonempty_iff_ne_empty, ne.def, ←disjoint_iff_inter_eq_empty],
+    exact λ hDI, hD.dep (hI₀.indep.subset (hDI.subset_right_of_subset_union hDss))},
+
+  obtain ⟨x,hx⟩ := heD,
+  apply hI x hx.2,
+  refine mem_of_mem_of_subset (hD.subset_cl_diff_singleton x hx.1) _,
+  rw [←cl_union_cl_right_eq_cl_union, ←hI₀.cl, cl_union_cl_right_eq_cl_union],
+  refine cl_subset_cl_of_subset _ (diff_subset_iff.mpr (hDss.trans _)),
+  rw [singleton_union, insert_union_distrib, insert_diff_singleton],
+  exact union_subset_union (subset_insert _ _) (subset_insert _ _),
+end
+
+lemma project_indep_of_union_basis_indep (hI₀ : M.basis I₀ C) (hdj : disjoint I I₀)
+(h_ind : M.indep (I ∪ I₀)) :
+  (M ⟋ C).indep I :=
+begin
+  simp_rw [indep_iff_not_mem_cl_diff_forall, project_cl_eq],
+  rw [indep_iff_not_mem_cl_diff_forall] at h_ind,
+  intros x hxI,
+  refine not_mem_subset _ (h_ind _ (or.inl hxI)),
+  rw [←cl_union_cl_right_eq_cl_union, ←hI₀.cl, cl_union_cl_right_eq_cl_union, union_diff_distrib,
+    diff_singleton_eq_self (disjoint_left.mp hdj hxI)],
+  exact rfl.subset,
+end
+
+lemma project_indep_iff_exists :
+  (M ⟋ C).indep I ↔ ∃ I₀, disjoint I I₀ ∧ M.basis I₀ C ∧ M.indep (I ∪ I₀) :=
+begin
+  refine ⟨λ h, _,λ h, _⟩,
+  { obtain ⟨I₀, hI₀⟩ := M.exists_basis C,
+    refine ⟨I₀, disjoint_of_subset_right hI₀.subset (project_indep_disjoint_contract h), hI₀, _⟩,
+    exact union_indep_of_project_indep h hI₀},
+  obtain ⟨I₀, hII₀, hI₀, hu⟩ := h,
+  exact project_indep_of_union_basis_indep hI₀ hII₀ hu,
+end
+
+lemma project_indep_iff_forall :
+  (M ⟋ C).indep I ↔ disjoint I C ∧ ∀ I₀, M.basis I₀ C → M.indep (I ∪ I₀) :=
+begin
+  refine ⟨λ hI, ⟨project_indep_disjoint_contract hI, λ I₀ hI₀,
+    union_indep_of_project_indep hI hI₀⟩, _⟩,
+  rw project_indep_iff_exists,
+  rintro ⟨hdj, hbas⟩,
+  obtain ⟨I₀, hI₀⟩ := M.exists_basis C,
+  exact ⟨I₀, disjoint_of_subset_right hI₀.subset hdj, hI₀, hbas _ hI₀⟩,
+end
+
+lemma project_basis_of_basis (hI : M.basis I (X ∪ C)) (hIC : M.basis (I ∩ C) C) :
+  (M ⟋ C).basis (I \ C) X :=
+begin
+  simp_rw [basis_iff_indep_cl, project_cl_eq, diff_union_self, diff_subset_iff],
+  refine ⟨project_indep_of_union_basis_indep hIC _ _, _, _⟩,
+  { rw disjoint_iff_forall_ne, rintro x ⟨-,hxC⟩ y ⟨-,hyC⟩ rfl, exact hxC hyC},
+  { rw diff_union_inter, exact hI.indep},
+  { rw [←cl_union_cl_left_eq_cl_union, hI.cl, cl_union_cl_left_eq_cl_union,
+      union_assoc, union_self],
+    refine subset_trans (subset_union_left _ _) (M.subset_cl _)},
+  rw [union_comm],
+  exact hI.subset,
+end
+
+lemma union_basis_of_project_basis (hI : (M ⟋ C).basis I X) (hI₀ : M.basis I₀ C) :
+  M.basis (I ∪ I₀) (X ∪ C) :=
+begin
+  simp_rw [basis_iff_indep_cl],
+  refine ⟨union_indep_of_project_indep hI.indep hI₀, _,
+    union_subset_union hI.subset hI₀.subset⟩,
+  simp_rw [basis_iff_indep_cl, project_cl_eq] at hI,
+  rw [←cl_union_cl_right_eq_cl_union, hI₀.cl, cl_union_cl_right_eq_cl_union],
+  exact union_subset hI.2.1 ((subset_union_right _ _).trans (M.subset_cl _)),
+end
+
+lemma project_basis_iff_exists :
+  (M ⟋ C).basis I X ↔ ∃ I₀, disjoint I I₀ ∧ M.basis I₀ C ∧ M.basis (I ∪ I₀) (X ∪ C) :=
+begin
+  split,
+  { obtain ⟨I₀, hI₀⟩ := M.exists_basis C,
+    exact λ h, ⟨I₀, disjoint_of_subset_right hI₀.subset (project_indep_disjoint_contract h.indep),
+      hI₀, union_basis_of_project_basis h hI₀⟩},
+  rintro ⟨I₀, hII₀, hI₀C, hb⟩,
+  have h'' := hI₀C.eq_of_subset_indep (hb.indep.inter_right C)
+      (subset_inter (subset_union_right _ _) hI₀C.subset) (inter_subset_right _ _),
+
+  convert project_basis_of_basis hb (h'' ▸ hI₀C),
+  have h' := inter_union_diff (I ∪ I₀) C,
+
+  refine subset_antisymm (subset_diff.mpr ⟨subset_union_left _ _,_⟩) (diff_subset_iff.mpr _),
+  { rw disjoint_iff_forall_ne,
+    rintro x hxI hy hyC rfl,
+    exact hII₀.ne_of_mem hxI (((set.ext_iff.mp h'') x).mpr ⟨or.inl hxI, hyC⟩) rfl},
+  exact (union_subset_union_right _ hI₀C.subset).trans_eq (union_comm _ _),
+end
+
+lemma project_basis_iff_forall :
+  (M ⟋ C).basis I X ↔ disjoint I (M.cl C) ∧ ∀ I₀, M.basis I₀ C → M.basis (I ∪ I₀) (X ∪ C) :=
+begin
+  split,
+  { exact λ hI, ⟨project_indep_disjoint_cl_contract hI.indep, λ I₀ hI₀,
+      union_basis_of_project_basis hI hI₀⟩},
+  rintro ⟨hIdj, h⟩,
+  rw project_basis_iff_exists,
+  obtain ⟨I₀, hI₀⟩ := M.exists_basis C,
+  exact ⟨I₀, disjoint_of_subset_right (hI₀.subset.trans (M.subset_cl _)) hIdj, hI₀, h _ hI₀⟩,
+end
+
+@[simp] lemma coe_r_project (M : matroid E) (C X : set E) :
+  ((M ⟋ C).r X : ℤ) = M.r (X ∪ C) - M.r C :=
+begin
+  obtain ⟨I,hI⟩ := (M ⟋ C).exists_basis X,
+  obtain ⟨I₀,hI₀⟩ := M.exists_basis C,
+  obtain ⟨h1,h2⟩  := project_basis_iff_forall.mp hI,
+  specialize h2 _ hI₀,
+
+  rw [←hI.r, hI.indep.r, ←h2.r, ←hI₀.r, hI₀.indep.r, h2.indep.r, ncard_union_eq],
+  {rw [nat.cast_add], linarith},
+  exact disjoint_of_subset_right (hI₀.subset.trans (M.subset_cl _)) h1,
+end
+
+lemma indep.project_indep_iff (hI₀ : M.indep I₀) : 
+  (M ⟋ I₀).indep I ↔ disjoint I I₀ ∧ M.indep (I ∪ I₀) :=
+begin
+  simp_rw [project_indep_iff_exists],
+  split,
+  { rintro ⟨J, hdj, hJ, hIJ⟩,
+    have := hI₀.eq_of_basis hJ, subst this,
+    exact ⟨hdj, hIJ⟩},
+  rintro ⟨hdj, hI⟩,
+  exact ⟨I₀, hdj, hI₀.basis_self, hI⟩,
+end
+
+lemma indep_of_project_indep (h : (M ⟋ C).indep I) :
+  M.indep I :=
+h.weak_image (project_weak_image _ _)
+
+lemma project_cl_eq_project (M : matroid E) (C : set E) :
+  M ⟋ (M.cl C) = M ⟋ C  :=
+eq_of_cl_eq_cl_forall (λ X, by simp_rw [project_cl_eq, cl_union_cl_right_eq_cl_union])
+
+lemma basis.project_eq_project (hI : M.basis I X) :
+  M ⟋ I = M ⟋ X :=
+by rw [←project_cl_eq_project, ←M.project_cl_eq_project X, hI.cl]
+
+@[simp] lemma project_loops_eq :
+  (M ⟋ C).cl ∅ = M.cl C :=
+by rw [project_cl_eq, empty_union]
+
+lemma loop_of_project_iff :
+  (M ⟋ C).loop e ↔ e ∈ M.cl C :=
+by rw [loop_iff_mem_cl_empty, project_cl_eq, empty_union]
+
+lemma loop_of_project_mem_cl (he : e ∈ M.cl C) :
+  (M ⟋ C).loop e :=
+loop_of_project_iff.mpr he
+
+lemma loop_of_project_mem (he : e ∈ C) :
+  (M ⟋ C).loop e :=
+loop_of_project_iff.mpr (mem_of_mem_of_subset he (M.subset_cl _))
+
+lemma project_eq_of_loops (h : C ⊆ M.cl ∅) :
+  (M ⟋ C) = M :=
+by rw [←project_cl_eq_project, cl_eq_loops_of_subset h, project_cl_eq_project, project_empty]
+
+lemma project_eq_self_iff_subset_loops :
+  M ⟋ C = M ↔ C ⊆ M.cl ∅ :=
+begin
+  refine ⟨λ h e heC, _, project_eq_of_loops⟩, 
+  rw [←h, project_loops_eq],
+  exact (M.subset_cl C) heC, 
+end    
+
+@[simp] lemma project_elem (M : matroid E) (e : E) : M ⟋ e = M ⟋ ({e} : set E) := rfl 
+
+lemma indep_project_singleton_iff (he : M.nonloop e) (heI : e ∉ I) :
+  (M ⟋ e).indep I ↔ M.indep (insert e I) :=
+begin
+  rw [project_elem], 
+  rw [←indep_singleton] at he, 
+  split, 
+  { intro h, 
+    have := he.project_indep_iff, 
+    rw [this, union_singleton] at h, 
+    exact h.2},
+  intro h, 
+  rw [he.project_indep_iff, union_singleton, disjoint_singleton_right], 
+  exact ⟨heI, h⟩,    
+end 
+
+lemma r_project_singleton_add_one (he : ¬M.loop e) (X : set E) :
+  (M ⟋ e).r X  + 1 = M.r (insert e X) :=
+by {zify, rw [project_elem, coe_r_project, nonloop_iff_r.mp he], simp}
+
+lemma coe_r_project_singleton (he : ¬M.loop e) (X : set E) :
+  ((M ⟋ e).r X : ℤ) = M.r (insert e X) - 1 :=
+by {rw ←r_project_singleton_add_one he X, simp}
+
+lemma not_mem_of_indep_project_singleton (h : (M ⟋ e).indep I) :
+  e ∉ I :=
+(loop_of_project_mem (mem_singleton e)).not_mem_indep h
+
+end project
+
+section loopify
+
+/-- The loopification of `D` in a matroid `M` is obtained from `M` by turning all elements of `D`
+  into loops. Not very mathematically natural, but often more convenient than deletion because the
+  underlying type remains the same. -/
+def loopify (M : matroid E) (D : set E) :
+  matroid E :=
+{ base := (λ I, M.basis I Dᶜ),
+  exists_base' := M.exists_basis Dᶜ,
+  base_exchange' := λ I₁ I₂ h₁ h₂ e, h₁.exchange h₂,
+  maximality := 
+  begin
+  sorry 
+    -- rintro I X ⟨B, hB, hIB⟩ hIX,  
+    -- intros X I B, simp, 
+  end }
+
+instance {E : Type*} [finite E] : has_del (matroid E) (set E) := ⟨matroid.loopify⟩ 
+instance {E : Type*} [finite E] : has_del (matroid E) E := ⟨λ M e, M.loopify {e}⟩  
+
+@[simp] lemma loopify_elem (M : matroid E) (e : E) : M ⟍ e = M ⟍ ({e} : set E) := rfl 
+
+@[simp] lemma base_loopify_iff :
+  (M ⟍ D).base B ↔ M.basis B Dᶜ  :=
+iff.rfl
+
+@[simp] lemma indep_loopify_iff :
+  (M ⟍ D).indep I ↔ disjoint I D ∧ M.indep I :=
+begin
+  simp_rw [indep_iff_subset_base, base_loopify_iff],
+  split,
+  { rintro ⟨B, hB, hIB⟩,
+    exact ⟨disjoint_of_subset_left hIB (subset_compl_iff_disjoint_right.mp hB.subset),
+      hB.indep.exists_base_supset.imp (λ B h, ⟨h.1, hIB.trans h.2⟩)⟩},
+  rintro ⟨hID, B, hB, hIB⟩,
+  obtain ⟨B', hIB', hB'⟩ :=
+    (hB.indep.subset hIB).subset_basis_of_subset (subset_compl_iff_disjoint_right.mpr hID),
+  use [B',hB',hIB'],
+end
+
+lemma indep_of_loopify_indep (h : (M ⟍ D).indep I ):
+  M.indep I :=
+(indep_loopify_iff.mp h).2
+
+lemma loopify_weak_image (M : matroid E) (D : set E):
+  M ⟍ D ≤w M :=
+begin
+  intros I hI,
+  rw indep_loopify_iff at hI,
+  exact hI.2,
+end
+
+@[simp] lemma loopify_empty (M : matroid E):
+  M ⟍ (∅ : set E) = M  :=
+eq_of_indep_iff_indep_forall (λ I, by simp)
+
+lemma circuit_loopify_iff :
+  (M ⟍ D).circuit C ↔ (M.circuit C ∧ disjoint C D) ∨ ∃ e ∈ D, C = {e} :=
+begin
+  simp_rw [circuit_def, indep_loopify_iff, not_and, exists_prop],
+  split,
+  { rintro ⟨h₁, h₂⟩,
+    obtain (h | ⟨e,heC,heD⟩) := (C ∩ D).eq_empty_or_nonempty,
+    { left,
+      rw ←disjoint_iff_inter_eq_empty at h,
+      exact ⟨⟨h₁ h, λ I hIC, (h₂ I hIC).2⟩,h⟩},
+      refine or.inr ⟨e,heD, _⟩,
+      obtain (hss | rfl) := (singleton_subset_iff.mpr heC).ssubset_or_eq, swap, refl,
+      have hcon := (h₂ _ hss).1,
+      rw [disjoint_singleton_left] at hcon,
+      exact (hcon heD).elim},
+  rintro (⟨⟨hdep, h⟩,hdj⟩  | ⟨e,heD,rfl⟩),
+  { exact ⟨λ _, hdep, λ I hIC, ⟨disjoint_of_subset_left hIC.subset hdj, h I hIC⟩⟩},
+  refine ⟨λ h, (disjoint_singleton_left.mp h heD).elim, λ I hI, _⟩,
+  rw ssubset_singleton_iff at hI,
+  subst hI,
+  exact ⟨empty_disjoint _, M.empty_indep⟩,
+end
+
+lemma circuit_loopify_iff_of_disjoint (hC : disjoint C D) :
+  (M ⟍ D).circuit C ↔ M.circuit C :=
+begin
+  rw [circuit_loopify_iff],
+  refine ⟨λ h, h.elim (and.left) _,λ h, (or.inl ⟨h,hC⟩)⟩,
+  rintro ⟨e,heD,rfl⟩,
+  refine h.elim (and.left) (false.elim ∘ _),
+  rintro ⟨f,hfD,hef⟩,
+  rw [hef, disjoint_singleton_left] at hC,
+  exact hC hfD,
+end
+
+@[simp] lemma loopify_cl_eq (D X : set E):
+  (M ⟍ D).cl X = M.cl (X \ D) ∪ D :=
+begin
+  ext e,
+  simp_rw [mem_cl_iff_exists_circuit, circuit_loopify_iff],
+  split,
+  { rintro (heX | ⟨C, ⟨⟨hC,hCD⟩ | ⟨f,hfD,rfl⟩,hC'⟩⟩),
+    { exact (em (e ∈ D)).elim or.inr (λ heD,
+        or.inl (mem_of_mem_of_subset (⟨heX, heD⟩ : e ∈ X \ D) (M.subset_cl _) ))},
+    { refine or.inl (mem_of_mem_of_subset (hC.subset_cl_diff_singleton e hC'.1)
+        (M.cl_subset_cl_of_subset _)),
+      rw [subset_diff],
+      exact ⟨hC'.2, disjoint_of_subset_left (diff_subset _ _) hCD⟩},
+    rw ←mem_singleton_iff.mp hC'.1 at hfD,
+    exact or.inr hfD},
+
+  by_cases heD : e ∈ D,
+  { exact λ _, or.inr ⟨{e}, or.inr ⟨_,heD,rfl⟩, mem_singleton_of_eq rfl, by simp⟩},
+  rintro (heX | heD'), swap, exact (heD heD').elim,
+
+  rw mem_cl_iff_exists_circuit at heX,
+  obtain ( heXD | ⟨C, hC, heC, hCX⟩) := heX,
+  { exact or.inl ((diff_subset _ _) heXD)},
+  refine (em (e ∈ X)).elim or.inl (λ heX, or.inr _),
+  refine ⟨C, or.inl ⟨hC, _⟩, heC, hCX.trans (diff_subset _ _)⟩,
+
+  rw [←inter_union_diff C {e}, disjoint_union_left, inter_singleton_eq_of_mem heC,
+    disjoint_singleton_left],
+  rw subset_diff at hCX,
+  exact ⟨heD, hCX.2⟩,
+end
+
+@[simp] lemma loop_loopify_iff :
+  (M ⟍ D).loop e ↔ M.loop e ∨ e ∈ D :=
+by { simp_rw [loop_iff_mem_cl_empty, loopify_cl_eq, empty_diff], refl }
+
+@[simp] lemma nonloop_loopify_iff :
+  (M ⟍ D).nonloop e ↔ M.nonloop e ∧ e ∉ D :=
+by simp_rw [←not_loop_iff, loop_loopify_iff, not_or_distrib] 
+
+lemma loopified_subset_loops (M : matroid E) (D : set E) :
+  D ⊆ (M ⟍ D).cl ∅ :=
+by {rw [loopify_cl_eq], exact subset_union_right _ _}
+
+lemma loop_of_loopify (h : e ∈ D) :
+  (M ⟍ D).loop e :=
+by {rw loop_iff_mem_cl_empty, exact M.loopified_subset_loops D h}
+
+@[simp] lemma loopify_nonloops (M : matroid E) (D : set E) :
+  ((M ⟍ D).cl ∅)ᶜ  = (M.cl ∅)ᶜ \ D :=
+by { ext, simp_rw [mem_diff, mem_compl_iff, ←loop_iff_mem_cl_empty, ←not_or_distrib, not_iff_not, 
+  loop_loopify_iff] }
+
+lemma basis_loopify_iff :
+  (M ⟍ D).basis I X ↔ disjoint I D ∧ M.basis I (X \ D) :=
+begin
+  simp_rw [basis_iff, indep_loopify_iff],
+  split,
+  { rintro ⟨⟨hdj, hI⟩, hIX, h⟩,
+    exact ⟨hdj, hI, (subset_diff.mpr ⟨hIX, hdj⟩), λ J hJ hIJ hJX,
+     h J ⟨(disjoint_of_subset_left hJX (disjoint_sdiff_left)),hJ⟩
+      hIJ (hJX.trans (diff_subset _ _))⟩},
+  rintro ⟨hdj,hI,hIXD,h⟩,
+  exact ⟨⟨hdj,hI⟩, hIXD.trans (diff_subset _ _), λ J h' hIJ hJX, h _ h'.2 hIJ
+    (subset_diff.mpr ⟨hJX, h'.1⟩)⟩,
+end
+
+lemma basis_loopify_iff_of_disjoint (h : disjoint X D) :
+  (M ⟍ D).basis I X ↔ M.basis I X :=
+begin
+  rw [basis_loopify_iff],
+  exact ⟨λ hI,
+    hI.2.basis_subset (hI.2.subset.trans (diff_subset _ _)) (subset_diff.mpr ⟨subset.rfl, h⟩),
+  λ hI, ⟨disjoint_of_subset_left hI.subset h, hI.basis_subset
+    (subset_diff.mpr ⟨hI.subset,disjoint_of_subset_left hI.subset h⟩) (diff_subset _ _)⟩⟩,
+end
+
+@[simp] lemma r_loopify :
+  (M ⟍ D).r X = M.r (X \ D) :=
+begin
+  obtain ⟨I, hI⟩ := (M ⟍ D).exists_basis X,
+  rw [←hI.r, hI.indep.r],
+  rw [basis_loopify_iff] at hI,
+  rw [←hI.2.r, hI.2.indep.r],
+end
+
+lemma loopify_eq_of_loops (h : D ⊆ M.cl ∅) :
+  M ⟍ D = M :=
+begin
+  refine eq_of_indep_iff_indep_forall (λ I, _),
+  rw [indep_loopify_iff],
+  refine ⟨and.right, λ hI, ⟨disjoint_of_subset_right h hI.disjoint_loops,hI⟩⟩,
+end
+
+lemma loopify_eq_self_iff_subset_loops :
+  M ⟍ D = M ↔ D ⊆ M.cl ∅ :=
+begin
+  refine ⟨λ h e heD, _, loopify_eq_of_loops⟩,
+  rw [←h, loopify_cl_eq],
+  exact or.inr heD,
+end
+
+lemma r_loopify_of_disjoint (h : disjoint X D) :
+  (M ⟍ D).r X = M.r X :=
+by rw [r_loopify, sdiff_eq_left.mpr h]
+
+@[simp] lemma loopify_loopify (M : matroid E) (D D' : set E) :
+  M ⟍ D ⟍ D' = M ⟍ (D ∪ D') :=
+begin
+  refine eq_of_indep_iff_indep_forall (λ I, _),
+  rw [indep_loopify_iff, indep_loopify_iff, indep_loopify_iff, ←and_assoc, and_comm (disjoint _ _)],
+  convert iff.rfl,
+  rw [disjoint_union_right],
+end
+
+lemma loopify_loopify_comm (M : matroid E) (D D' : set E) :
+  M ⟍ D ⟍ D' = M ⟍ D' ⟍ D :=
+by rw [loopify_loopify, union_comm, loopify_loopify]
+
+lemma not_mem_of_indep_loopify_singleton (h : (M ⟍ ({e} : set E)).indep I) :
+  e ∉ I :=
+(loop_of_loopify (mem_singleton e)).not_mem_indep h
+
+end loopify
+
+
+
+
+section pseudominor
+
+lemma project_loopify_swap (M : matroid E) (C D : set E) :
+  M ⟋ C ⟍ D = M ⟍ (D \ C) ⟋ C :=
+begin
+  refine eq_of_cl_eq_cl_forall (λ X, _),
+  simp only [project_cl_eq, loopify_cl_eq],
+  rw [union_diff_distrib, sdiff_sdiff_cancel_right, @diff_eq_compl_inter _ D C,
+    @diff_eq_compl_inter _ X (Cᶜ ∩ D), compl_inter, compl_compl, inter_distrib_right,
+    union_right_comm, union_eq_right_iff_subset.mpr (inter_subset_left _ _), ←diff_eq_compl_inter,
+    union_comm C, union_eq_union_iff_left],
+  refine ⟨_,(inter_subset_right _ _).trans (subset_union_right _ _)⟩,
+  rw [←diff_eq_compl_inter],
+  nth_rewrite 0 [←inter_union_diff D C],
+  refine union_subset
+    ((inter_subset_right _ _).trans (subset_union_of_subset_left _ _)) (subset_union_right _ _),
+  exact (subset_union_right _ _).trans (M.subset_cl _),
+end
+
+lemma loopify_project_swap (M : matroid E) (C D : set E) :
+  M ⟍ D ⟋ C = M ⟋ (C \ D) ⟍ D :=
+begin
+  rw [project_loopify_swap, sdiff_sdiff_cancel_right],
+  nth_rewrite 0 ←inter_union_diff C D,
+  rw [union_comm, ←project_project],
+  apply project_eq_of_loops,
+  simp only [project_cl_eq, empty_union, loopify_cl_eq, sdiff_idem],
+  exact (inter_subset_right _ _).trans (subset_union_right _ _),
+end
+
+lemma project_loopify_comm (M : matroid E) {C D : set E} (hCD : disjoint C D) :
+  M ⟋ C ⟍ D = M ⟍ D ⟋ C :=
+by {convert project_loopify_swap _ _ _, rwa [eq_comm, sdiff_eq_left, disjoint.comm]}
+
+lemma project_loopify_eq_self_iff_subset_loops :
+  M ⟋ C ⟍ D = M ↔ C ∪ D ⊆ M.cl ∅ :=
+begin
+  refine ⟨λ h, _,λ h, _⟩,
+  { rw ←h,
+    simp only [loopify_cl_eq, empty_diff, project_cl_eq, empty_union, union_subset_iff,
+      subset_union_right, and_true],
+    exact subset_union_of_subset_left (M.subset_cl _) _},
+  rw [loopify_eq_self_iff_subset_loops.mpr, project_eq_self_iff_subset_loops.mpr],
+  { exact (subset_union_left _ _).trans h},
+  simp only [project_cl_eq, empty_union],
+  exact (subset_union_right _ _).trans (h.trans (M.cl_mono (empty_subset C))),
+end
+
+/-- a pminor (pseudominor) of a matroid M is a matroid on the same ground set arising
+-- from loopifications and/or projections of M  -/
+def pminor (N M : matroid E) :=
+  ∃ (C D : set E), N = M ⟋ C ⟍ D
+
+def strict_pminor (N M : matroid E) :=
+  pminor N M ∧ N ≠ M
+
+infix ` ≤p ` :75 :=  matroid.pminor
+
+infix ` <p ` :75 :=  matroid.strict_pminor
+
+lemma strict_pminor.pminor (h : N <p M) :
+  N ≤p M :=
+h.1
+
+lemma strict_pminor.ne (h : N <p M) :
+  N ≠ M :=
+h.2
+
+lemma pminor.strict_pminor_of_ne (h : N ≤p M) (hne : N ≠ M) :
+  N <p M :=
+⟨h,hne⟩
+
+lemma pminor.weak_image (h : N ≤p M) :
+  N ≤w M :=
+by {obtain ⟨C,D,rfl⟩ := h, exact (loopify_weak_image _ _).trans (project_weak_image _ _)}
+
+lemma project_pminor (M : matroid E) (C : set E) :
+  M ⟋ C ≤p M :=
+⟨C, ∅, by simp⟩
+
+lemma loopify_pminor (M : matroid E) (D : set E) :
+  M ⟍ D ≤p M :=
+⟨∅, D, by simp⟩
+
+lemma project_loopify_pminor (M : matroid E) (C D : set E) :
+  M ⟋ C ⟍ D ≤p M :=
+⟨C,D,rfl⟩
+
+lemma loopify_project_pminor (M : matroid E) (C D : set E) :
+  M ⟍ D ⟋ C ≤p M :=
+⟨C \D,D, by {rw loopify_project_swap}⟩
+
+/-- This doesn't include co-independence of `D`. TODO -/
+lemma exists_canonical_pminor_of_pminor (h : N ≤p M) :
+  ∃ C D, N = M ⟋ C ⟍ D ∧ M.indep C ∧ disjoint D (M.cl C) :=
+begin
+  obtain ⟨C', D', rfl⟩ := h,
+  obtain ⟨C, hC⟩ := M.exists_basis C',
+  refine ⟨C, D' \ M.cl C, _, hC.indep, disjoint_sdiff_left⟩ ,
+  nth_rewrite 0 ←inter_union_diff D' (M.cl C),
+  rw [hC.project_eq_project, union_comm, ←loopify_loopify, loopify_eq_self_iff_subset_loops,
+    loopify_cl_eq, empty_diff, project_cl_eq, empty_union, hC.cl],
+  exact (inter_subset_right _ _).trans (subset_union_left _ _),
+end
+
+lemma pminor_trans {M₀ M₁ M₂ : matroid E} (h₀ : M₀ ≤p M₁) (h₁ : M₁ ≤p M₂) :
+  M₀ ≤p M₂ :=
+begin
+  obtain ⟨C₁,D₁,rfl, hC₁,hD₁⟩ := exists_canonical_pminor_of_pminor h₁,
+  obtain ⟨C₀,D₀,rfl, hC₀,hD₀⟩ := exists_canonical_pminor_of_pminor h₀,
+
+  have hdj : disjoint (C₀ ∪ C₁) (D₀ ∪ D₁),
+  { rw [disjoint_union_right, disjoint.comm],
+    split,
+    { refine disjoint_of_subset_right _ hD₀,
+      rw [loopify_cl_eq, project_cl_eq, union_subset_iff],
+      split,
+      { nth_rewrite 0 ←inter_union_diff C₀ D₁,
+        rw [union_comm],
+        exact union_subset_union ((subset_union_left _ _).trans (M₂.subset_cl _))
+            (inter_subset_right _ _)},
+      exact subset_union_of_subset_left ((subset_union_right _ _).trans (M₂.subset_cl _)) _},
+    rw [disjoint_union_left],
+    refine ⟨_, (disjoint_of_subset_left (M₂.subset_cl _) hD₁.symm)⟩,
+    simp only [indep_loopify_iff] at hC₀,
+    exact hC₀.1},
+
+  rw [project_loopify_comm, project_loopify_comm, project_loopify_comm, project_project,
+     loopify_loopify, ←project_loopify_comm],
+  { exact ⟨_,_,rfl⟩},
+  { rwa [union_comm, union_comm D₁]},
+  { exact disjoint_of_subset (subset_union_right _ _) (subset_union_left _ _) hdj},
+  { exact disjoint_of_subset (subset_union_right _ _) (subset_union_right _ _) hdj},
+  exact disjoint_of_subset (subset_union_left _ _) (subset_union_left _ _) hdj,
+end
+
+lemma pminor_antisymm (h : N ≤p M) (h' : M ≤p N) :
+  M = N :=
+h'.weak_image.antisymm h.weak_image
+
+lemma pminor.eq_of_loops_subset_loops (h : N ≤p M) (h_loops : N.cl ∅ ⊆ M.cl ∅) :
+  N = M :=
+begin
+  obtain ⟨C, D, rfl⟩:= h,
+  rw project_loopify_eq_self_iff_subset_loops,
+  simp only [loopify_cl_eq, project_cl_eq, empty_diff, empty_union] at *,
+  exact (union_subset_union_left D (M.subset_cl C)).trans h_loops,
+end
+
+lemma strict_pminor_of_project_nonloop (he : ¬M.loop e) :
+  M ⟋ e <p M :=
+begin
+  refine (project_pminor M {e}).strict_pminor_of_ne (λ h, he _),
+  rwa [project_eq_self_iff_subset_loops, singleton_subset_iff, ←loop_iff_mem_cl_empty] at h,
+end
+
+lemma strict_pminor_of_loopify_nonloop (he : ¬M.loop e) :
+  M ⟍ e <p M :=
+begin
+  refine (loopify_pminor M {e}).strict_pminor_of_ne (λ h, he _),
+  rwa [loopify_eq_self_iff_subset_loops, singleton_subset_iff, ←loop_iff_mem_cl_empty] at h,
+end
+
+lemma strict_pminor_of_project_loopify_r_ne_zero (h : M.r (C ∪ D) ≠ 0) :
+  M ⟋ C ⟍ D <p M :=
+begin
+  refine (project_loopify_pminor _ _ _).strict_pminor_of_ne
+    (λ hC, h (r_eq_zero_iff_subset_loops.mpr _)),
+  rwa [project_loopify_eq_self_iff_subset_loops] at hC,
+end
+
+lemma strict_pminor_of_project_r_ne_zero (h : M.r (C) ≠ 0) :
+  M ⟋ C <p M :=
+begin
+  refine (project_pminor _ _).strict_pminor_of_ne (λ hC, h (r_eq_zero_iff_subset_loops.mpr _)),
+  rwa [project_eq_self_iff_subset_loops] at hC,
+end
+
+lemma pminor.loops_supset_loops (h : N ≤p M) :
+  M.cl ∅ ⊆ N.cl ∅ :=
+begin
+  obtain ⟨C,D,rfl⟩ := h,
+  simp only [loopify_cl_eq, empty_diff, project_cl_eq, empty_union],
+  exact subset_union_of_subset_left (M.cl_mono (empty_subset C)) _,
+end
+
+lemma pminor.nonloops_subset_nonloops (h : N ≤p M) :
+  N.nonloops ⊆ M.nonloops :=
+by { simp_rw [nonloops_eq_compl_cl_empty, compl_subset_compl], exact h.loops_supset_loops } 
+
+lemma strict_pminor.nonloops_ssubset_nonloops (h : N <p M) :
+  N.nonloops ⊂ M.nonloops :=
+begin
+  refine (h.pminor.nonloops_subset_nonloops).ssubset_of_ne (λ he, h.ne _),
+  rw [nonloops_eq_compl_cl_empty, nonloops_eq_compl_cl_empty, compl_inj_iff] at he,
+  exact h.pminor.eq_of_loops_subset_loops he.subset,
+end
+
+end pseudominor
+
+end matroid
+
+
+-- lemma project_makes_loops (M : matroid E) (C : set E) : loops M ∪ C ⊆ loops (M ⟋ C)  :=
+-- by rw [←rank_zero_iff_subset_loops, project_r, union_assoc, union_self,
+--         union_comm, rank_eq_rank_union_rank_zero C (rank_loops M), sub_self]
+
+-- lemma loop_of_project (M : matroid E )(he : e ∈ C) : (M ⟋ C).is_loop e :=
+-- loop_iff_mem_loops.mpr (mem_of_mem_of_subset (by {exact or.inr he}) (project_makes_loops M C))
+
+-- lemma projected_set_rank_zero (M : matroid E) (C : set E) : (M ⟋ C).r C = 0 :=
+-- by rw [project_r, union_self, sub_self]
+
+-- lemma projected_set_union_rank_zero (M : matroid E) (C : set E){X : set E} (hX : M.r X = 0) :
+--   (M ⟋ C).r (X ∪ C) = 0 :=
+-- by rwa [project_r, union_assoc, union_self, union_comm, rank_eq_rank_union_rank_zero, sub_self]
+
+-- lemma project_rank_zero_eq (h : M.r C = 0) : M ⟋ C = M :=
+-- by {ext X, rw [project_r, rank_eq_rank_union_rank_zero X h, h, sub_zero]}
+
+-- lemma project_rank_zero_of_rank_zero (C : set E) (hX : M.r X = 0) : (M ⟋ C).r X = 0 :=
+-- by {apply rank_eq_zero_of_le_zero, rw ←hX, apply project_is_weak_image}
+
+-- lemma project_nonloops_eq (C : set E): (M ⟋ C).nonloops = M.nonloops \ M.cl C :=
+-- begin
+--   ext x,
+--   rw [mem_diff, ← nonloop_iff_mem_nonloops, ← nonloop_iff_mem_nonloops, nonloop_iff_r, project_r,
+--     nonmem_cl_iff_r, union_comm],
+--   refine ⟨λ h, ⟨by_contra (λ hn, _), by linarith⟩, λ h, by linarith [h.2]⟩,
+--   rw [← loop_iff_not_nonloop, loop_iff_r] at hn,
+--   rw [rank_eq_rank_union_rank_zero _ hn, sub_self] at h,
+--   exact zero_ne_one h,
+-- end
+
+-- lemma indep_union_project_set_of_project_indep
+-- (hX : is_indep (M ⟋ C) X) (hC : is_indep M C) :
+-- is_indep M (X ∪ C) :=
+-- by {simp_rw [indep_iff_r, project_r] at *,
+--     linarith [M.R1 (X ∪ C), size_modular X C, size_nonneg (X ∩ C)]}
+
+-- lemma project_nonloop_fewer_nonloops (he : M.is_nonloop e): (M ⟋ {e}).nonloops ⊂ M.nonloops :=
+-- begin
+--   simp_rw [nonloops_eq_compl_loops],
+--   apply ssubset_compl_commpl.mpr,
+--   rw ssubset_iff_subset_ne,
+--   refine ⟨subset.trans (subset_union_left _ _) (project_makes_loops M {e}), λ hn, _⟩,
+--   rw ext_iff at hn,
+--   have h' := (not_iff_not.mpr (hn e)).mp (nonloop_iff_not_mem_loops.mp he),
+--   exact h' (loop_iff_mem_loops.mp (loop_of_project M (mem_singleton e))),
+-- end
+
+-- lemma indep_of_project_indep (h: is_indep (M ⟋ C) X) : is_indep M X :=
+-- indep_of_weak_image_indep (project_is_weak_image M C) h
+
+-- lemma project_as_project_to (M : matroid E) (C : set E) : (M ⟋ C) = M.project_to Cᶜ :=
+-- by rw [project_to, compl_compl]
+
+-- lemma project_to_r (M : matroid E) (R X : set E) : (M.project_to R).r X = M.r (X ∪ Rᶜ) - M.r Rᶜ :=
+-- by rw [project_to, project_r]
+
+-- lemma indep_project_iff : (M ⟋ C).is_indep X ↔ M.is_indep X ∧ M.r (X ∪ C) = M.r X + M.r C :=
+-- begin
+--   rw [indep_iff_r,project_r, indep_iff_r],
+--   refine ⟨λ h, ⟨_,_⟩, λ h, _⟩,
+--   { refine le_antisymm (M.rank_le_size _) _, rw ←h, linarith [rank_subadditive M X C]},
+--   { refine le_antisymm (M.rank_subadditive X C) _,
+--     rw (by linarith : M.r (X ∪ C) = M.r C + size X),
+--     linarith [M.rank_le_size X], },
+--   rw [←h.1, h.2], simp,
+-- end
+
+-- lemma flat_of_flat_project (h : (M ⟋ C).is_flat F) : M.is_flat F :=
+-- flat_of_quotient_flat (project_is_quotient _ _) h
+
+-- lemma flat_project_iff : (M ⟋ C).is_flat F ↔ M.is_flat F ∧ C ⊆ F :=
+-- begin
+--   refine ⟨λ h, ⟨flat_of_flat_project h,_⟩, λ h, _⟩,
+--   { refine subset.trans _ (loops_subset_flat _ h),
+--     rw ←rank_zero_iff_subset_loops,
+--     apply projected_set_rank_zero, },
+--   simp_rw [flat_iff_r, project_r, union_comm F C, subset_iff_union_eq_left.mp h.2],
+--   intros Y hFY,
+--   suffices : M.r F < M.r Y, linarith [rank_mono_union_left M Y C],
+--   exact h.1 _ hFY,
+-- end
+
+-- lemma point_project_nonloop_iff { e : E } (he : M.is_nonloop e){X : set E}:
+--   (M ⟋ {e}).is_point X ↔ M.is_line X ∧ e ∈ X :=
+-- begin
+--   dsimp only  [is_point, is_line, is_rank_k_flat, project_r],
+--   rw [flat_project_iff, rank_nonloop he, singleton_subset_iff],
+--   split,
+--   { rintros ⟨⟨hF,he⟩,hX⟩,
+--     rw [union_mem_singleton he] at hX,
+--     exact ⟨⟨hF, eq_add_of_sub_eq hX⟩, he⟩ },
+--   rintros ⟨⟨hF, hX⟩, he⟩,
+--   rw [union_mem_singleton he, hX],
+--   tidy,
+-- end
+
+-- end project
+
+-- section loopify
+
+-- variables {E : Type*} [fintype E] {e f : E} {M : matroid E} {X Y D C I R S : set E}
+
+-- /-- Replace D with loops to get a matroid on the same ground set. Often more
+-- convenient than deleting D -/
+-- def loopify (M : matroid E) (D : set E) : matroid E :=
+-- { r := λ X, M.r (X \ D),
+--   R0 := λ X, M.R0 _,
+--   R1 := λ X, by linarith [M.R1 (X \ D), size_diff_le_size X D],
+--   R2 := λ X Y hXY, M.rank_mono (diff_subset_diff_left hXY),
+--   R3 := λ X Y, by {simp only [diff_eq], rw [inter_distrib_right, inter_distrib_inter_left],
+--                     linarith [M.rank_submod (X ∩ Dᶜ) (Y ∩ Dᶜ)], }}
+
+-- infix ` ⟍ ` :75 :=  matroid.loopify
+
+-- /-- loopify all elements of M outside R -/
+-- def lrestrict (M : matroid E) (R : set E) : matroid E := M ⟍ (Rᶜ)
+
+-- infix ` ‖ `  :75 :=  matroid.lrestrict
+
+-- @[simp] lemma loopify_r (M : matroid E) (D X : set E) : (M ⟍ D).r X = M.r (X \ D) := rfl
+-- @[simp] lemma loopify_empty (M : matroid E) : M ⟍ ∅ = M :=
+-- by { ext X, rw [loopify_r, diff_empty]}
+
+-- lemma loopify_is_weak_image (M : matroid E) (D : set E) :
+--   M ⟍ D ≤ M :=
+-- λ X, rank_mono_diff _ _ _
+
+-- lemma loopify_loopify (M : matroid E) (D D' : set E) :
+--    M ⟍ D ⟍ D' = M ⟍ (D ∪ D') :=
+-- by {ext X, simp [diff_eq, ←inter_assoc, inter_right_comm]}
+
+-- lemma loopify_loops_eq (M : matroid E) (D : set E) :
+--   M.loops ∪ D = (M ⟍ D).loops :=
+-- begin
+--   refine subset.antisymm _ (λ x hx, _),
+--   { rw [←rank_zero_iff_subset_loops, loopify_r, rank_zero_iff_subset_loops], tidy,},
+
+--   rw [← loop_iff_mem_loops, loop_iff_r, loopify_r] at hx,
+--   by_contra hn,
+--   rw [mem_union_eq, not_or_distrib, ← nonloop_iff_not_mem_loops, nonloop_iff_r] at hn,
+--   have hxD : {x} \ D = {x},
+--   { ext,
+--     simp only [mem_singleton_iff, and_iff_left_iff_imp, mem_diff],
+--     rintro rfl,
+--     exact hn.2},
+--   rw [hxD,hn.1] at hx,
+--   exact one_ne_zero hx,
+-- end
+
+-- lemma loops_subset_loopify_loops_eq (M : matroid E)(D : set E):
+--   M.loops ⊆ (M ⟍ D).loops :=
+-- by {rw ← loopify_loops_eq, apply subset_union_left}
+
+-- lemma loop_of_loopify (M : matroid E) (he : e ∈ D) :
+--   (M ⟍ D).is_loop e :=
+-- by {rw [loop_iff_mem_loops, ← loopify_loops_eq], exact or.inr he}
+
+-- lemma loopify_nonloops_eq (M : matroid E) (D : set E):
+--   (M ⟍ D).nonloops = M.nonloops \ D :=
+-- by rw [nonloops_eq_compl_loops, nonloops_eq_compl_loops, ← loopify_loops_eq, compl_union, diff_eq]
+
+-- lemma loopify_nonloop_fewer_nonloops (he : M.is_nonloop e):
+--   (M ⟍ {e}).nonloops ⊂ M.nonloops :=
+-- begin
+--   simp_rw [nonloops_eq_compl_loops],
+--   apply ssubset_compl_commpl.mpr,
+--   rw ← loopify_loops_eq,
+--   exact ssubset_of_add_nonmem_iff.mp (nonloop_iff_not_mem_loops.mp he),
+-- end
+
+-- lemma loopify_rank_zero_eq (h : M.r D = 0) :
+--   M ⟍ D = M :=
+-- by {ext X, rw [loopify_r, rank_eq_rank_diff_rank_zero X h]}
+
+-- lemma loopified_set_rank_zero (M : matroid E) (D : set E) :
+--   (M ⟍ D).r D = 0 :=
+-- by rw [loopify_r, set.diff_self, rank_empty]
+
+-- lemma loopified_set_union_rank_zero (M : matroid E) (D : set E){X : set E} (h: M.r X = 0) :
+--   (M ⟍ D).r (X ∪ D) = 0 :=
+-- by {rw [loopify_r, union_diff_right], exact rank_zero_of_subset_rank_zero (diff_subset _ _) h}
+
+-- lemma loopify_rank_zero_of_rank_zero (D : set E)(hX : M.r X = 0) :
+--   (M ⟍ D).r X = 0 :=
+-- by {apply rank_eq_zero_of_le_zero, rw ←hX, apply loopify_is_weak_image}
+
+-- lemma loopify_rank_of_disjoint (M : matroid E) (h : D ∩ X = ∅) :
+--   (M ⟍ D).r X = M.r X :=
+-- by {rw loopify_r, congr, rwa [inter_comm, disjoint_iff_diff_eq_left] at h}
+
+-- lemma indep_of_loopify_indep (hX : is_indep (M ⟍ D) X) :
+--   is_indep M X :=
+-- indep_of_weak_image_indep (loopify_is_weak_image M D) hX
+
+
+-- lemma indep_loopify_iff :
+--   (M ⟍ D).is_indep X ↔ M.is_indep X ∧ X ∩ D = ∅ :=
+-- by rw [loopify_as_lrestrict, indep_lrestrict_iff, subset_compl_iff_disjoint]
+
+-- lemma indep_of_indep_lrestrict (hI : (M ‖ R).is_indep I) :
+--   M.is_indep I :=
+-- (indep_lrestrict_iff.mp hI).1
+
+-- lemma indep_lrestrict_subset_is_indep
+-- (hSR: S ⊆ R) (hI: (M ‖ S).is_indep I ) :
+--   (M ‖ R).is_indep I :=
+-- by {simp_rw [indep_lrestrict_iff] at *, exact ⟨hI.1, subset.trans hI.2 hSR⟩}
+
+-- lemma lrestrict_eq_lrestrict_iff {M N : matroid E}:
+--   M ‖ S = N ‖ S ↔ (∀ X ⊆ S, M.r X = N.r X) :=
+-- begin
+--   refine ⟨λ h, λ X hX, _, λ h, _⟩,
+--   { rw [← (subset_iff_inter_eq_left.mp hX), ← lrestrict_r, ← lrestrict_r, h]},
+--   ext Y : 2 ,
+--   rw [lrestrict_r, lrestrict_r, h _ (inter_subset_right _ _)],
+-- end
+
+-- end loopify
+
+-- section pminor
+
+-- variables {E : Type*} [fintype E] { M N : matroid E } {C D : set E}
+
+-- /-- a pminor (pseudominor) of a matroid M is a matroid on the same ground set arising
+-- from loopifications and/or projections of M  -/
+-- def is_pminor_of (N M : matroid E) :=
+--   ∃ C D, N = M ⟋ C ⟍ D
+
+-- lemma pr_is_pminor (M : matroid E) (C : set E):
+--   (M ⟋ C).is_pminor_of M :=
+-- ⟨C, ∅, by simp⟩
+
+-- lemma lp_is_pminor (M : matroid E) (D : set E):
+--   (M ⟍ D).is_pminor_of M :=
+-- ⟨∅, D, by simp⟩
+
+-- lemma pr_lp_eq_lp_pr (M : matroid E) (C D : set E) :
+--   M ⟋ C ⟍ D = M ⟍ (D \ C) ⟋ C :=
+-- by {ext X, simp only [loopify_r, project_r], convert rfl; {ext, simp, tauto! }}
+
+-- lemma lp_pr_eq_pr_lp (M : matroid E) (C D : set E) :
+--   M ⟍ D ⟋ C = M ⟋ (C \ D) ⟍ D :=
+-- by {ext X, simp only [loopify_r, project_r], convert rfl; {ext, simp, tauto! }}
+
+-- lemma rank_zero_of_lp_pr (M : matroid E) (C D : set E) :
+--   (M ⟍ D ⟋ C).r (C ∪ D) = 0 :=
+-- begin
+--   apply rank_zero_of_union_rank_zero, apply projected_set_rank_zero,
+--   apply project_rank_zero_of_rank_zero, apply loopified_set_rank_zero,
+-- end
+
+-- lemma rank_zero_of_pr_lp (M : matroid E) (C D : set E) :
+--   (M ⟋ C ⟍ D).r (C ∪ D) = 0 :=
+-- begin
+--   apply rank_zero_of_union_rank_zero,
+--   apply loopify_rank_zero_of_rank_zero, apply projected_set_rank_zero,
+--   apply loopified_set_rank_zero,
+-- end
+
+-- lemma pminor_iff_exists_lp_pr_disjoint {N M : matroid E} :
+--   N.is_pminor_of M ↔ ∃ C D, C ∩ D = ∅ ∧ N = M ⟍ D ⟋ C :=
+-- begin
+--   split, rintros ⟨C,D,h⟩, refine ⟨C,D \ C, ⟨by simp ,_⟩ ⟩, rwa ←pr_lp_eq_lp_pr,
+--   rintros ⟨C,D,hCD,h⟩, refine ⟨C \ D, D, _⟩, rwa ←lp_pr_eq_pr_lp,
+-- end
+
+-- lemma pminor_iff_exists_pr_lp_disjoint {N M : matroid E} :
+--   N.is_pminor_of M ↔ ∃ C D, C ∩ D = ∅ ∧ N = M ⟋ C ⟍ D :=
+-- begin
+--   split, swap, rintros ⟨C,D,hCD,h⟩, exact ⟨C, D, h⟩,
+--   rintros ⟨C,D,h⟩, refine ⟨C,D \ C, ⟨by simp ,_⟩ ⟩,
+--   rw [h, ←loopify_rank_zero_eq (_ : (M ⟋ C ⟍ (D \ C)).r (C ∩ D) = 0), loopify_loopify],
+--   { congr, ext, simp, tauto!, },
+--   refine rank_zero_of_subset_rank_zero _ (rank_zero_of_pr_lp _ _ _),
+--   intro x, simp, tauto,
+-- end
+
+-- end pminor
+
+-- end matroid
